Iris/Iris/Algebra/Csum.lean
@@ -52,8 +52,8 @@ theorem dist_eqv [OFE α] [OFE β] {n} : Equivalence (Csum.Dist (α := α) (β :
 instance [OFE α] [OFE β] : OFE (Csum α β) where
   Dist := Csum.Dist
   dist_eqv := dist_eqv
-  eq_dist {x y} := by
-    cases x <;> cases y <;> simp [Csum.Dist, (eq_dist (SI := Nat))]
+  eq_dist' {x y} := by
+    cases x <;> cases y <;> simp [Csum.Dist, (eq_dist _)]
   dist_lt {n x y m} hn hlt := by
     cases x <;> cases y <;> first | exact OFE.Dist.lt hn hlt | exact hn.elim | trivial
 
