Iris/Iris/Algebra/Lib/ExclAuth.lean
@@ -79,7 +79,7 @@ theorem agreeN {a b : A} (h : ✓{n} (●E a) • ◯E b) : a ≡{n}≡ b :=
 
 @[rocq_alias excl_auth_agree]
 theorem agree {a b : A} (h : ✓ (●E a) • ◯E b) : a = b :=
-  OFE.eq_dist.mpr fun _ => agreeN (Valid.validN h)
+  (OFE.eq_dist _).mpr fun _ => agreeN (Valid.validN h)
 
 #rocq_ignore excl_auth_agree_L "Use agree"
 
