Iris/Iris/Algebra/List.lean
@@ -29,14 +29,14 @@ theorem forall₂_eq_of_forall₂_dist : ∀ {l k : List α},
   | [], _ :: _, h => nomatch h 0
   | _ :: _, [], h => nomatch h 0
   | _ :: _, _ :: _, h => List.cons_eq_cons.mpr
-    ⟨eq_dist.mpr (fun n => (List.forall₂_cons.mp <| h n).1),
+    ⟨(eq_dist _).mpr (fun n => (List.forall₂_cons.mp <| h n).1),
      forall₂_eq_of_forall₂_dist fun n => (List.forall₂_cons.mp (h n)).2⟩
 
 @[rocq_alias list_ofe_mixin]
 instance : OFE (List α) where
   Dist n := List.Forall₂ (Dist n)
   dist_eqv := List.Forall₂.equivalence dist_eqv
-  eq_dist := ⟨fun h _ => h ▸ (List.Forall₂.rfl .refl), forall₂_eq_of_forall₂_dist⟩
+  eq_dist' := ⟨fun h _ => h ▸ (List.Forall₂.rfl .refl), forall₂_eq_of_forall₂_dist⟩
   dist_lt h hlt := h.imp fun hab => hab.lt hlt
 #rocq_ignore listO "Use List"
 #rocq_ignore list_dist "Local Dist instance; folded into Lean's OFE (List α) instance."
