Iris/Iris/Algebra/View.lean
@@ -79,11 +79,11 @@ instance instOFE : OFE (View R) where
     symm H := ⟨H.1.symm, H.2.symm⟩
     trans H1 H2 := ⟨H1.1.trans H2.1, H1.2.trans H2.2⟩
   }
-  eq_dist {x y} := by
+  eq_dist' {x y} := by
     refine ⟨fun H _ => H ▸ ⟨.rfl, .rfl⟩, fun H => ?_⟩
     obtain ⟨xa, xf⟩ := x; obtain ⟨ya, yf⟩ := y
     simp only [View.mk.injEq]
-    exact ⟨eq_dist.mpr fun n => (H n).1, eq_dist.mpr fun n => (H n).2⟩
+    exact ⟨(eq_dist _).mpr fun n => (H n).1, (eq_dist _).mpr fun n => (H n).2⟩
   dist_lt H Hn := ⟨dist_lt H.1 Hn, dist_lt H.2 Hn⟩
 
 #rocq_ignore viewO "Use the plain View type and typeclass inference"
@@ -127,12 +127,12 @@ theorem auth_dist_inj [UCMRA B] {q1 q2 : DFrac} {a1 a2 : A} {n}
 @[rocq_alias view_auth_inj]
 theorem auth_eqv_inj [UCMRA B] {q1 q2 : DFrac} {a1 a2 : A}
     (H : (●V{q1} a1 : View R) = ●V{q2} a2) : q1 = q2 ∧ a1 = a2 := by
-  refine ⟨(auth_dist_inj (n := 0) H.dist).1, (OFE.eq_dist (SI := Nat)).mpr fun n => ?_⟩
+  refine ⟨(auth_dist_inj (n := 0) H.dist).1, (OFE.eq_dist _).mpr fun n => ?_⟩
   exact (auth_dist_inj H.dist).2
 
 @[rocq_alias view_frag_inj]
 theorem frag_eqv_inj [UCMRA B] {b1 b2 : B}
-    (H : (◯V b1 : View R) = ◯V b2) : b1 = b2 := (OFE.eq_dist (SI := Nat)).mpr fun _ => H.dist (SI := Nat).2
+    (H : (◯V b1 : View R) = ◯V b2) : b1 = b2 := (OFE.eq_dist _).mpr fun _ => H.dist (SI := Nat).2
 
 @[rocq_alias view_frag_dist_inj]
 theorem dist_of_frag_dist [UCMRA B] {b1 b2 : B} {n} (H : (◯V b1 : View R) ≡{n}≡ ◯V b2) :
@@ -436,7 +436,7 @@ theorem dist_of_validN_auth (H : ✓{n} ((●V{dq1} a1 : View R) • ●V{dq2} a
 @[rocq_alias view_auth_dfrac_op_inv_L]
 theorem eq_of_valid_auth
     (H : ✓ ((●V{dq1} a1 : View R) • ●V{dq2} a2)) : a1 = a2 :=
-  OFE.eq_dist.mpr fun _ => dist_of_validN_auth H.validN
+  (OFE.eq_dist _).mpr fun _ => dist_of_validN_auth H.validN
 
 @[rocq_alias view_auth_dfrac_validN]
 theorem auth_validN_iff : ✓{n} (●V{dq} a : View R) ↔ ✓{n}dq ∧ R n a UCMRA.unit :=
@@ -497,7 +497,7 @@ theorem auth_op_auth_valid_iff : ✓ ((●V{dq1} a1 : View R) • ●V{dq2} a2) 
   refine ⟨fun H => ?_, fun H n => ?_⟩
   · simp [valid, CMRA.op, op, optionOp, CMRA.ValidN, ValidN] at H
     let Hn n := dist_of_validN_auth <| H n
-    refine ⟨(H 0).1, OFE.eq_dist.mpr Hn, fun n => ?_⟩
+    refine ⟨(H 0).1, (OFE.eq_dist _).mpr Hn, fun n => ?_⟩
     · rcases (H n) with ⟨_, _, Hl, H⟩
       apply mono H ?_ CMRA.incN_unit n.le_refl
       apply toAgree.inj (Hl.symm.trans ?_)
@@ -551,7 +551,7 @@ open CMRA in
 theorem auth_inc_auth_op_frag_iff : ((●V{dq1} a1 : View R) ≼ (●V{dq2} a2 : View R) • ◯V b) ↔ (dq1 ≼ dq2 ∨ dq1 = dq2) ∧ a1 = a2 := by
   refine ⟨fun H => ⟨?_, ?_⟩, fun H => ?_⟩
   · exact auth_incN_auth_op_frag_iff (n := 0) |>.mp (CMRA.incN_of_inc _ H) |>.1
-  · refine (OFE.eq_dist (SI := Nat)).mpr (fun n => ?_)
+  · refine (OFE.eq_dist _).mpr (fun n => ?_)
     exact auth_incN_auth_op_frag_iff |>.mp (CMRA.incN_of_inc _ H) |>.2
   · rcases H with ⟨(⟨q, Hq⟩|Hq), Ha⟩
     · calc (●V{dq1} a1 : View R)
